feat(keyrings): annotate RawRSAKeyring

src/AwsCryptographicMaterialProviders/Keyrings/RawRSAKeyring.dfy
@@ -35,10 +35,18 @@ module
   type ValidRSAPublicKey = key: RSAEncryption.PublicKey | key.Valid()  witness *
   type ValidRSAPrivateKey = key: RSAEncryption.PrivateKey | key.Valid() witness *
 
+  type ValidRawRSAKeyring = keyring: RawRSAKeyring |
+    //= compliance/framework/raw-rsa-keyring.txt#2.1.1
+    //= type=TODO
+    //# -  Raw RSA keyring MUST NOT accept a key namespace of "aws-kms".
+    && UTF8.Decode(keyring.keyNamespace).UnwrapOr("aws-kms") != "aws-kms"
+    && (keyring.publicKey.Some? || keyring.privateKey.Some?)
+    witness *
+    
   function method paddingSchemeToMinStrengthBits(
     padding: RSAEncryption.PaddingMode
   ): (strength: RSAEncryption.StrengthBits)
-    //Reverse of RSAEncryption.GetBtyes
+    //  Reverse of RSAEncryption.GetBtyes
     ensures RSAEncryption.GetBytes(strength) == RSAEncryption.MinStrengthBytes(padding)
   {
     ((RSAEncryption.MinStrengthBytes(padding) * 8) - 7) as RSAEncryption.StrengthBits
@@ -46,6 +54,10 @@ module
 
   //TODO :: What external method can we use to verify a pem is a pem?
   //TODO :: Where should this method live? Probably in AwsCryptographicMaterialProviders
+  //= compliance/framework/raw-rsa-keyring.txt#2.5.3
+  //# The raw RSA keyring SHOULD support loading PEM
+  //# encoded PKCS #8 PrivateKeyInfo structures
+  //# (https://tools.ietf.org/html/rfc5958#section-2) as private keys.
   method importPrivateKey(
     pem: seq<uint8>,
     padding: RSAEncryption.PaddingMode
@@ -95,7 +107,14 @@ module
     );
     return Success(key);
   }
-    
+
+  //= compliance/framework/raw-rsa-keyring.txt#2.5.2
+  //= type=TODO
+  //# The raw RSA keyring SHOULD support loading PEM
+  //# encoded X.509 SubjectPublicKeyInfo structures
+  //# (https://tools.ietf.org/html/rfc5280#section-4.1) as public keys.
+
+  
   class RawRSAKeyring
     extends Keyring.VerifiableInterface, Crypto.IKeyring
   {
@@ -105,11 +124,48 @@ module
     const privateKey: Option<seq<uint8>>
     const paddingScheme: RSAEncryption.PaddingMode
 
+    //= compliance/framework/raw-rsa-keyring.txt#2.5
+    //= type=implication
+    //# On keyring initialization, the caller MUST provide the following:
+    //#*  Key Namespace (./keyring-interface.md#key-namespace)
+    //#*  Key Name (./keyring-interface.md#key-name)
+    //#*  Padding Scheme (Section 2.5.1)
+    //#*  Public Key (Section 2.5.2) and/or Private Key (Section 2.5.3)
     constructor (
       namespace: UTF8.ValidUTF8Bytes,
       name: UTF8.ValidUTF8Bytes,
+      
+      //= compliance/framework/raw-rsa-keyring.txt#2.5.2
+      //= type=TODO
+      //# The public key MUST follow the RSA specification for public keys
+      //# (Section 2.4.2).
+      // NOTE: section 2.4.2 is a lie,
+      // See https://datatracker.ietf.org/doc/html/rfc8017#section-3.1 instead
+      // NOTE: A sequence of uint8 is NOT how a public key is stored according to the RFC linked, though it is how the libraries we use define them
       publicKey: Option<seq<uint8>>,
+      
+      //= compliance/framework/raw-rsa-keyring.txt#2.5.3
+      //= type=TODO
+      //# The private key MUST follow the RSA specification for private keys
+      //# (Section 2.4.2).
+      // NOTE: section 2.4.2 is a lie,
+      // See https://datatracker.ietf.org/doc/html/rfc8017#section-3.2 instead
+      // NOTE: A sequence of uint8s is NOT how a public key is stored according to the RFC linked, though it is how the libraries we use define them
       privateKey: Option<seq<uint8>>,
+
+      //= compliance/framework/raw-rsa-keyring.txt#2.5.3
+      //= type=TODO
+      //# The
+      //# private key SHOULD contain all Chinese Remainder Theorem (CRT)
+      //# components (public exponent, prime factors, CRT exponents, and CRT
+      //# coefficient).
+      // NOTE: What? Shouldn't the above be on the Cryptographic library?
+      // i.e.: BouncyCastle, pyca, etc.?
+
+      //= compliance/framework/raw-rsa-keyring.txt#2.5.1
+      //= type=implication
+      //# This value MUST correspond with one of the supported padding schemes
+      //# (Section 2.5.1.1).
       paddingScheme: RSAEncryption.PaddingMode
     )
       requires |namespace| < UINT16_LIMIT
@@ -126,7 +182,11 @@ module
       this.publicKey := publicKey;
       this.privateKey := privateKey;
     }
-    
+
+    //= compliance/framework/raw-rsa-keyring.txt#2.6.1
+    //= type=implication
+    //# OnEncrypt MUST take encryption materials (structures.md#encryption-
+    //# materials) as input.
     method OnEncrypt(input: Crypto.OnEncryptInput)
       returns (res: Result<Crypto.OnEncryptOutput, string>)
       ensures
@@ -136,31 +196,115 @@ module
           input.materials,
           res.value.materials
         )
+
+     //= compliance/framework/raw-rsa-keyring.txt#2.6.1
+     //= type=implication
+     //# OnEncrypt MUST fail if this keyring does not have a specified public
+     //# key (Section 2.5.2).
+     ensures
+       this.publicKey.None? || |this.publicKey.Extract()| == 0
+     ==>
+       res.Failure?
+
+     //= compliance/framework/raw-rsa-keyring.txt#2.6.1
+     //= type=implication
+     //# If the encryption materials (structures.md#encryption-materials) do
+     //# not contain a plaintext data key, OnEncrypt MUST generate a random
+     //# plaintext data key and set it on the encryption materials
+     //# (structures.md#encryption-materials).
+     ensures
+       && input.materials.plaintextDataKey.None?
+       && res.Success?
+     ==>
+       res.value.materials.plaintextDataKey.Some?
+
+     //= compliance/framework/raw-rsa-keyring.txt#2.6.1
+     //= type=implication
+     //# If RSA encryption was successful, OnEncrypt MUST return the input
+     //# encryption materials (structures.md#encryption-materials), modified
+     //# in the following ways:
+     //#*  The encrypted data key list has a new encrypted data key added,
+     //#   constructed as follows:
+     ensures
+       && res.Success?
+     ==>
+       |res.value.materials.encryptedDataKeys| == |input.materials.encryptedDataKeys| + 1
+
+     //= compliance/framework/raw-rsa-keyring.txt#2.6.1
+     //= type=implication
+     //# The keyring MUST NOT derive a public key from a
+     //# specified private key (Section 2.5.3).
+     // NOTE: Attempting to proove this by stating that a Keyring
+     // without a public key but with a private key will not encrypt
+     ensures
+       this.privateKey.Some? && this.publicKey.None?
+     ==>
+       res.Failure?
     {
       :- Need(
         this.publicKey.Some? && |this.publicKey.Extract()| > 0,
         "A RawRSAKeyring without a public key cannot provide OnEncrypt"
       );
-
+      
       var materials := input.materials;
       var suite := GetSuite(materials.algorithmSuiteId);
       
       var newPlaintextDataKey :- Random.GenerateBytes(suite.encrypt.keyLength as int32);
 
+      //= compliance/framework/raw-rsa-keyring.txt#2.6.1
+      //# If the encryption materials (structures.md#encryption-materials) do
+      //# not contain a plaintext data key, OnEncrypt MUST generate a random
+      //# plaintext data key and set it on the encryption materials
+      //# (structures.md#encryption-materials).
       var plaintextDataKey :=
         if materials.plaintextDataKey.Some? && |materials.plaintextDataKey.Extract()| > 0
         then materials.plaintextDataKey.value
         else newPlaintextDataKey;
-      
+
+      //= compliance/framework/raw-rsa-keyring.txt#2.6.1
+      //# The keyring MUST attempt to encrypt the plaintext data key in the
+      //# encryption materials (structures.md#encryption-materials) using RSA.
+      //# The keyring performs RSA encryption (Section 2.4.2) with the
+      //# following specifics:
       var ciphertext :- RSAEncryption.EncryptExtern(
+        //= compliance/framework/raw-rsa-keyring.txt#2.6.1
+        //#*  This keyring's padding scheme (Section 2.5.1.1) is the RSA padding
+        //#   scheme.
         this.paddingScheme,
+
+        //= compliance/framework/raw-rsa-keyring.txt#2.6.1
+        //#*  This keyring's public key (Section 2.5.2) is the RSA public key.
         this.publicKey.Extract(),
+
+        //= compliance/framework/raw-rsa-keyring.txt#2.6.1
+        //#*  The plaintext data key is the plaintext input to RSA encryption.
         plaintextDataKey
       );
-        
+
+      //= compliance/framework/raw-rsa-keyring.txt#2.6.1
+      //# If RSA encryption was successful, OnEncrypt MUST return the input
+      //# encryption materials (structures.md#encryption-materials), modified
+      //# in the following ways:
+      //#*  The encrypted data key list has a new encrypted data key added,
+      //#   constructed as follows:
       var edk: Crypto.EncryptedDataKey := Crypto.EncryptedDataKey(
+
+        //= compliance/framework/raw-rsa-keyring.txt#2.6.1
+        //#  -  The key provider ID (structures.md#key-provider-id) field is
+        //#     this keyring's key namespace (keyring-interface.md#key-
+        //#     namespace).
         keyProviderId := this.keyNamespace,
+
+        //= compliance/framework/raw-rsa-keyring.txt#2.6.1
+        //#  -  The key provider information (structures.md#key-provider-
+        //#     information) field is this keyring's key name (keyring-
+        //#     interface.md#key-name).
         keyProviderInfo := this.keyName,
+
+        //= compliance/framework/raw-rsa-keyring.txt#2.6.1
+        //#  -  The ciphertext (structures.md#ciphertext) field is the
+        //#     ciphertext output by the RSA encryption of the plaintext data
+        //#     key.
         ciphertext := ciphertext
       );
         
@@ -171,6 +315,11 @@ module
       return Success(Crypto.OnEncryptOutput(materials := r));      
     }
 
+    //= compliance/framework/raw-rsa-keyring.txt#2.6.2
+    //= type=implication
+    //# OnDecrypt MUST take decryption materials (structures.md#decryption-
+    //# materials) and a list of encrypted data keys
+    //# (structures.md#encrypted-data-key) as input.
     method OnDecrypt(input: Crypto.OnDecryptInput)
       returns (res: Result<Crypto.OnDecryptOutput, string>)
       ensures res.Success?
@@ -179,6 +328,25 @@ module
           input.materials,
           res.value.materials
         )
+          
+      //= compliance/framework/raw-rsa-keyring.txt#2.6.2
+      //= type=implication
+      //# OnDecrypt MUST fail if this keyring does not have a specified private
+      //# key (Section 2.5.3).
+      ensures
+        this.privateKey.None? || |this.privateKey.Extract()| == 0
+      ==>
+        res.Failure?
+
+      //= compliance/framework/raw-rsa-keyring.txt#2.6.2
+      //= type=implication
+      //# If the decryption materials already contain a plaintext data key, the
+      //# keyring MUST fail and MUST NOT modify the decryption materials
+      //# (structures.md#decryption-materials).
+      ensures
+        input.materials.plaintextDataKey.Some?
+      ==>
+        res.Failure?
     {
       :- Need(
         this.privateKey.Some? && |this.privateKey.Extract()| > 0,
@@ -191,9 +359,19 @@ module
         "Keyring received decryption materials that already contain a plaintext data key."
       );
 
+      //= compliance/framework/raw-rsa-keyring.txt#2.6.2
+      //# The keyring MUST attempt to decrypt the input encrypted data keys, in
+      //# list order, until it successfully decrypts one.
       var i := 0;
       while i < |input.encryptedDataKeys|
-        invariant forall prevIndex :: 0 <= prevIndex < i ==> prevIndex < |input.encryptedDataKeys|
+        invariant
+          forall prevIndex :: 0 <= prevIndex < i
+        ==>
+          && prevIndex < |input.encryptedDataKeys|
+      //     && (
+      //       || !ShouldDecryptEDK(input.encryptedDataKeys[prevIndex])
+      //       || DecryptFailed(input.encryptedDataKeys[prevIndex])
+      //     )
       {
         if ShouldDecryptEDK(input.encryptedDataKeys[i]) {
           var edk := input.encryptedDataKeys[i];
@@ -202,21 +380,67 @@ module
             this.privateKey.Extract(),
             edk.ciphertext
           );
-  
+
+          //= compliance/framework/raw-rsa-keyring.txt#2.6.2
+          //# If any decryption succeeds, this keyring MUST immediately return the
+          //# input decryption materials (structures.md#decryption-materials),
+          //# modified in the following ways:
           if decryptResult.Success? {
-            var r :- Materials.DecryptionMaterialsAddDataKey(materials, decryptResult.Extract());
+            //= compliance/framework/raw-rsa-keyring.txt#2.6.2
+            //#*  The output of RSA decryption is set as the decryption material's
+            //#   plaintext data key.
+            var r :- Materials.DecryptionMaterialsAddDataKey(
+              materials,
+              decryptResult.Extract()
+            );
             return Success(Crypto.OnDecryptOutput(materials := r));
           }
         }
         i := i + 1;
       }
+      //= compliance/framework/raw-rsa-keyring.txt#2.6.2
+      //# If no decryption succeeds, the keyring MUST fail and MUST NOT modify
+      //# the decryption materials (structures.md#decryption-materials).
       return Failure("Unable to decrypt data key: No Encrypted Data Keys found to match.");
     }
 
-    predicate method ShouldDecryptEDK(edk: Crypto.EncryptedDataKey) {
+
+    predicate method ShouldDecryptEDK(edk: Crypto.EncryptedDataKey)
+      //= compliance/framework/raw-rsa-keyring.txt#2.6.2
+      //= type=implication
+      //# For each encrypted data key, the keyring MUST attempt to decrypt the
+      //# encrypted data key into plaintext using RSA if and only if the
+      //# following is true:
+      ensures
+        //= compliance/framework/raw-rsa-keyring.txt#2.6.2
+        //= type=implication
+        //#*  The encrypted data key's key provider information
+        //#   (structures.md#key-provider-information). has a value equal to
+        //#   this keyring's key name (keyring-interface.md#key-name).
+        && edk.keyProviderInfo == this.keyName
+        
+        //= compliance/framework/raw-rsa-keyring.txt#2.6.2
+        //= type=implication
+        //#*  The encrypted data key's key provider ID (structures.md#key-
+        //#   provider-id) has a value equal to this keyring's key namespace
+        //#   (keyring-interface.md#key-namespace).
+        && edk.keyProviderId == this.keyNamespace
+
+        && |edk.ciphertext| > 0
+      ==>
+        true
+    {
       && edk.keyProviderInfo == this.keyName
       && edk.keyProviderId == this.keyNamespace
       && |edk.ciphertext| > 0
+    }
+
+    // TODO: Complete predicate so that it can be used to prove that
+    // all previous attempted edk decryptions failed
+    predicate {:opaque} DecryptFailed(edk: Crypto.EncryptedDataKey)
+      requires this.privateKey.Some? && |this.privateKey.Extract()| > 0
+    {
+      true
     }
   }
 }
